Improve tacticts to support Snyder notation and doubles

src/basic.lean
@@ -136,27 +136,27 @@ begin
 end
 
 /-- Outer pencil marks capture the fact that a certain number appears in one of two places. -/
-def outer_pencil_mark (s : sudoku) (i j k l m : fin 9) : Prop :=
+def snyder (s : sudoku) (i j k l m : fin 9) : Prop :=
 s.f (i, j) = m ∨ s.f (k, l) = m
 
 /-- Inner pencil marks capture the fact that a certain cell contains one of two numbers. -/
-def inner_pencil_mark₂ (s : sudoku) (i j k l : fin 9) : Prop :=
+def double (s : sudoku) (i j k l : fin 9) : Prop :=
 s.f (i, j) = k ∨ s.f (i, j) = l
 
 /-- Inner pencil marks capture the fact that a certain cell contains one of three numbers. -/
-def inner_pencil_mark₃ (s : sudoku) (i j k l m : fin 9) : Prop :=
+def triple (s : sudoku) (i j k l m : fin 9) : Prop :=
 s.f (i, j) = k ∨ s.f (i, j) = l ∨ s.f (i, j) = m
 
 /-- The first (trivial) piece of sudoku theory: If there are two outer pencil marks relating two
     cells, then we get an inner pencil mark for those two numbers in both cells. -/
-lemma inner_left_of_outer {s : sudoku} {i j k l m n : fin 9} (h₀ : outer_pencil_mark s i j k l m)
-  (h₁ : outer_pencil_mark s i j k l n) (h₂ : m ≠ n) : inner_pencil_mark₂ s i j m n :=
-by { unfold inner_pencil_mark₂, tidy }
+lemma inner_left_of_outer {s : sudoku} {i j k l m n : fin 9} (h₀ : snyder s i j k l m)
+  (h₁ : snyder s i j k l n) (h₂ : m ≠ n) : double s i j m n :=
+by { unfold double, tidy }
 
 /-- The first (trivial) piece of sudoku theory: If there are two outer pencil marks relating two
     cells, then we get an inner pencil mark for those two numbers in both cells. -/
-lemma inner_right_of_outer {s : sudoku} {i j k l m n : fin 9} (h₀ : outer_pencil_mark s i j k l m)
-  (h₁ : outer_pencil_mark s i j k l n) (h₂ : m ≠ n) : inner_pencil_mark₂ s k l m n :=
-by { unfold inner_pencil_mark₂, tidy }
+lemma inner_right_of_outer {s : sudoku} {i j k l m n : fin 9} (h₀ : snyder s i j k l m)
+  (h₁ : snyder s i j k l n) (h₂ : m ≠ n) : double s k l m n :=
+by { unfold double, tidy }
 
 end sudoku
